MirrorCharge!/src/MirrorCharge/Java/TestPullConjunct.v
@@ -1,0 +1,30 @@
+Require Import MirrorCharge.Java.JavaType.
+Require Import MirrorCharge.Java.JavaFunc.
+
+Require Import MirrorCharge.SetoidRewrite.Base.
+Require Import MirrorCharge.SetoidRewrite.ILSetoidRewrite.
+Require Import MirrorCharge.SetoidRewrite.BILSetoidRewrite.
+Require Import MirrorCharge.SetoidRewrite.EmbedSetoidRewrite.
+
+Require Import MirrorCharge.RTac.PullConjunct.
+
+Require Import MirrorCharge.ModularFunc.BaseFunc.
+Require Import MirrorCharge.ModularFunc.ILogicFunc.
+Require Import MirrorCharge.ModularFunc.EmbedFunc.
+
+Require Import MirrorCore.Lambda.ExprCore.
+Require Import MirrorCore.RTac.RTac.
+
+Definition f (e : expr typ func) := match ilogicS e with Some (ilf_false _) => true | _ => false end.
+Definition PCT := PULLCONJUNCTL typ func subst f ilops.
+
+Set Printing Width 140.
+
+Definition goal1 : expr typ func := mkEntails tyProp 
+	(mkAnd tyProp (mkTrue tyProp) (mkFalse tyProp)) (mkTrue tyProp).
+
+Definition goal2 : expr typ func := mkEntails tyProp 
+	(mkAnd tyProp (mkAnd tyProp (mkTrue tyProp) (mkFalse tyProp)) (mkAnd tyProp (mkAnd tyProp (mkFalse tyProp) (mkTrue tyProp)) (mkFalse tyProp))) (mkTrue tyProp).
+
+Eval vm_compute in PCT CTop (SubstI.empty (expr := expr typ func)) goal1.
+Eval vm_compute in PCT CTop (SubstI.empty (expr := expr typ func)) goal2.
