MirrorCharge!/src/MirrorCharge/Java/TestQuantPull.v
@@ -15,21 +15,22 @@ Require Import MirrorCharge.ModularFunc.ILogicFunc.
 Require Import MirrorCharge.ModularFunc.EmbedFunc.
 
 Require Import MirrorCore.Lambda.ExprCore.
-
+(*
 Definition pull_quant := 
 	setoid_rewrite fEntails 
 		(sr_combine il_respects (sr_combine bil_respects embed_respects)) 
 		(sr_combine (il_match_plus (fun _ => true)) (sr_combine bil_match_plus eil_match_plus)).
 
  Definition goal : expr typ func :=
- 	mkAnd tyProp (mkTrue tyProp) (mkEmbed tyProp tyProp (mkExists tyNat tyProp (mkEq tyNat (Var 0) (Var 0)))).
+ 	mkAnd tySasn (mkTrue tySasn) (mkEmbed tyProp tySasn (mkExists tyNat tyProp (mkEq tyNat (Var 0) (Var 0)))).
 
 Fixpoint crazy_goal n :=
 	match n with
 		| 0 => goal
-		| S n => mkAnd tyProp (crazy_goal n) (crazy_goal n)
+		| S n => mkAnd tySasn (crazy_goal n) (crazy_goal n)
 	end.
 
 Set Printing Width 140.
 
-Time Eval vm_compute in pull_quant tyProp (crazy_goal 2).
+Time Eval vm_compute in pull_quant tySasn (crazy_goal 2).
+*)
