MirrorCharge!/src/MirrorCharge/PullConjunct/ILPullConjunct.v
@@ -1,0 +1,81 @@
+Require Import MirrorCore.Lambda.ExprCore.
+Require Import MirrorCore.Lambda.Red.
+Require Import MirrorCore.Lambda.ExprLift.
+Require Import MirrorCore.TypesI.
+
+Require Import ExtLib.Core.RelDec.
+
+Require Import MirrorCharge.SetoidRewrite.Base.
+Require Import MirrorCharge.ModularFunc.ILogicFunc.
+Require Import MirrorCharge.AutoSetoidRewrite.
+
+Require Import Charge.Logics.ILogic.
+
+Section ILPullConjunct.
+  Context {typ func : Type} {HIL : ILogicFunc typ func}.
+  Context {RType_typ : RType typ}.
+  Context {RelDec_func : RelDec (@eq (expr typ func))}.
+
+  Let Rbase := expr typ func.
+
+  Variable target : expr typ func -> bool.  
+
+Definition il_pull_conjunct_l (e : expr typ func) (_ : list (RG (expr typ func))) (rg : RG Rbase) : m (expr typ func) :=
+  match e with
+    | App (App a P) (App (App b Q) R) =>
+      match ilogicS (typ := typ) (func := expr typ func) a, ilogicS b with
+      	| Some (ilf_and l), Some (ilf_and _) =>
+      		match target Q with
+      			| true => rg_plus
+                   (rg_bind (unifyRG (@rel_dec (expr typ func) _ _) rg (RGflip (RGinj (fEntails l))))
+				      (fun _ => rg_ret (mkAnd l Q (mkAnd l P R))))
+				   (rg_bind (unifyRG (@rel_dec (expr typ func) _ _) rg (RGinj (fEntails l)))
+				      (fun _ => rg_ret (mkAnd l Q (mkAnd l P R))))      			
+      		    | _ => rg_fail
+      		end
+      	| _, _ => rg_fail
+      end
+    | _ => rg_fail
+  end.
+
+Definition il_pull_conjunct_r (e : expr typ func) (_ : list (RG (expr typ func))) (rg : RG Rbase) : m (expr typ func) :=
+  match e with
+    | App (App a (App (App b P) Q)) R =>
+      match ilogicS (typ := typ) (func := expr typ func) a, ilogicS b with
+      	| Some (ilf_and l), Some (ilf_and _) =>
+      		match target P with
+      			| true => rg_plus
+	               (rg_bind (unifyRG (@rel_dec (expr typ func) _ _) rg (RGflip (RGinj (fEntails l))))
+					 (fun _ => rg_ret (mkAnd l P (mkAnd l Q R))))
+				   (rg_bind (unifyRG (@rel_dec (expr typ func) _ _) rg (RGinj (fEntails l)))
+					 (fun _ => rg_ret (mkAnd l P (mkAnd l Q R))))      			
+      		    | _ => rg_fail
+      		end
+      	| _, _ => rg_fail
+      end
+    | _ => rg_fail
+  end.
+
+Definition il_pull_conjunct_sym (e : expr typ func) (_ : list (RG (expr typ func))) (rg : RG Rbase) : m (expr typ func) :=
+  match e with
+    | App (App a P) Q =>
+      match ilogicS (typ := typ) (func := expr typ func) a with
+      	| Some (ilf_and l) =>
+      		match target Q with
+      		  | true => rg_plus
+		                  (rg_bind (unifyRG (@rel_dec (expr typ func) _ _) rg (RGflip (RGinj (fEntails l))))
+				 		     (fun _ => rg_ret (mkAnd l Q P)))
+				 		  (rg_bind (unifyRG (@rel_dec (expr typ func) _ _) rg (RGinj (fEntails l)))
+						     (fun _ => rg_ret (mkAnd l Q P)))     
+      		  | _ => rg_fail
+      		end
+        | _ => rg_fail
+      end
+    | _ => rg_fail
+  end.  
+
+Definition il_pull_conjunct := sr_combine il_pull_conjunct_sym (sr_combine il_pull_conjunct_l il_pull_conjunct_r).
+
+End ILPullConjunct.
+
+Implicit Arguments il_pull_conjunct [[typ] [func] [HIL] [RelDec_func]].
