MirrorCharge!/src/MirrorCharge/RTac/PullConjunct.v
@@ -1,0 +1,71 @@
+Require Import ExtLib.Core.RelDec.
+
+Require Import MirrorCore.Lambda.Expr.
+Require Import MirrorCore.RTac.RTac.
+Require Import MirrorCore.STac.STac.
+Require Import MirrorCore.Subst.FMapSubst.
+Require Import MirrorCore.Lambda.ExprSubst.
+Require Import MirrorCore.Lambda.ExprUnify_simul.
+Require MirrorCore.syms.SymEnv.
+Require MirrorCore.syms.SymSum.
+
+Require Import MirrorCharge.ILogicFunc.
+Require Import MirrorCharge.ModularFunc.BaseFunc.
+Require Import MirrorCharge.ModularFunc.ILogicFunc.
+Require Import MirrorCharge.SetoidRewrite.Base.
+Require Import MirrorCharge.SetoidRewrite.ILSetoidRewrite.
+Require Import MirrorCharge.PullConjunct.ILPullConjunct.
+
+Require Import Charge.Logics.ILogic.
+
+Set Implicit Arguments.
+Set Strict Implicit.
+
+Section PullConjunct.
+  Context (typ func subst : Type).
+  Context {HIL : ILogicFunc typ func} {HB : BaseFunc typ func}.
+  Context {RelDec_func : RelDec (@eq (expr typ func))}.
+  Context {target : expr typ func -> bool}.
+  Context {RType_typ : RType typ}.
+  Context {HT : Typ2 RType_typ Fun}.
+  Context {RSym_func : RSym func}.
+  Context {ilogic : forall t : typ, option (ILogicOps (typD t))}.
+
+  Definition pull_conjunct := 
+	setoid_rewrite fEntails (sr_combine il_respects (il_respects_reflexive (ilogic := ilogic))) (il_pull_conjunct target).
+
+  Definition stac_pull_conjunct_l : stac typ (expr typ func) subst :=
+    fun tus tvs s hyps e =>
+      match e with
+        | App (App f L) R =>
+          match ilogicS f with
+	        | Some (ilf_entails l) =>
+	        	More nil nil s hyps (mkEntails l (pull_conjunct l L) R)
+	        | _ => More nil nil s hyps e
+	      end
+        | _ => More nil nil s hyps e
+      end.
+
+End PullConjunct.
+
+Implicit Arguments stac_pull_conjunct_l [[HIL] [HB] [RelDec_func] [RType_typ] [HT] [RSym_func]].
+
+Section PullConjunctTac.
+  Context {typ func subst : Type}.
+  Context {HIL : ILogicFunc typ func} {HB : BaseFunc typ func}.
+  Context {RelDec_func : RelDec (@eq (expr typ func))}.
+  Context {target : expr typ func -> bool}.
+  Context {SS : SubstI.Subst subst (expr typ func)}.
+  Context {SU : SubstI.SubstUpdate subst (expr typ func)}.
+  Context {RType_typ : RType typ}.
+  Context {HT : Typ2 RType_typ Fun}.
+  Context {RSym_func : RSym func}.
+  Context {ilogic : forall t : typ, option (ILogicOps (typD t))}.
+  
+  Definition PULLCONJUNCTL :=
+    (STAC_no_hyps (@ExprSubst.instantiate typ func) (stac_pull_conjunct_l typ func subst target ilogic)).
+
+End PullConjunctTac.
+
+Implicit Arguments PULLCONJUNCTL [[HIL] [HB] [RelDec_func] [SS] [SU] [RType_typ] [HT] [RSym_func]].
+
