MirrorCharge!/src/MirrorCharge/SetoidRewrite/ILSetoidRewrite.v
@@ -1,4 +1,5 @@
-Require Import MirrorCore.Lambda.ExprCore.
+Require Import MirrorCore.Lambda.Expr.
+Require Import MirrorCore.SymI.
 
 Require Import ExtLib.Core.RelDec.
 
@@ -7,10 +8,15 @@ Require Import MirrorCharge.ModularFunc.BaseFunc.
 Require Import MirrorCharge.ModularFunc.ILogicFunc.
 Require Import MirrorCharge.AutoSetoidRewrite.
 
+Require Import Charge.Logics.ILogic.
+
 Section ILSetoidRewrite.
 	Context {typ func : Type} {HIL : ILogicFunc typ func} {HB : BaseFunc typ func}.
-	Context {RelDec_func : RelDec (@eq (expr typ func))}.
-
+	Context {RelDec_func : RelDec (@eq (expr typ func))} {RType_typ : RType typ}.
+	Context {ilogic : forall t : typ, option (ILogicOps (typD t))}.
+	Context {HT : Typ2 RType_typ Fun}.
+	Context {RSym_func : RSym func}.
+	
 	Let Rbase := expr typ func.
 
   Definition il_respects (e : Rbase) (_ : list (RG Rbase))
@@ -41,9 +47,28 @@ Section ILSetoidRewrite.
 						                  (RGinj (fEntails l))))
 						                 
 				 (fun _ => rg_ret (fExists t l))
-		 | Some (ilf_true l) => rg_bind (unifyRG (@rel_dec (expr typ func) _ _) rg (RGinj (fEntails l)))
+(*		 | Some (ilf_true l) => rg_bind (unifyRG (@rel_dec (expr typ func) _ _) rg (RGinj (fEntails l)))
 			 	(fun _ => rg_ret (fTrue l))
+		 | Some (ilf_false l) => rg_bind (unifyRG (@rel_dec (expr typ func) _ _) rg (RGinj (fEntails l)))
+			 	(fun _ => rg_ret (fFalse l))*)
 		 | _ => rg_fail
 	 end.
 
+  Definition il_respects_reflexive (e : Rbase) (_ : list (RG Rbase))
+	   (rg : RG Rbase) : m (expr typ func) :=
+  	match typeof_expr nil nil e with
+      | Some t => match ilogic t with
+  				    | Some _ => rg_bind (unifyRG (@rel_dec (expr typ func) _ _) rg (RGinj (fEntails t)))
+								 	(fun _ => rg_ret e)
+  				    | None => rg_fail
+  				  end
+  	  | None => rg_fail
+  	end.
+(*
+	   rg_bind (unifyRG (@rel_dec (expr typ func) _ _) rg (RGinj (fEntails l)))
+	   	 (fun _ => rg_ret e).
+
+  Definition il_respects_reflexive := fold_right (fun t acc => sr_combine (il_respects_reflexive_aux t) acc) 
+  	(fun _ _ _ => rg_fail).
+*)
 End ILSetoidRewrite.
